first version of generators (no shrinking and no intra-component calls)

I2SFI/CompilerPBTests.v
@@ -25,36 +25,424 @@ Import GenLow GenHigh.
 (* Suppress some annoying warnings: *)
 Set Warnings "-extraction-opaque-accessed,-extraction".
 
-Instance show_intermediate_program : Show Intermediate.program :=
+Module DoNotation.
+Import ssrfun.
+Notation "'do!' X <- A ; B" :=
+  (bindGen A (fun X => B))
+  (at level 200, X ident, A at level 100, B at level 200).
+End DoNotation.
+Import DoNotation.
+
+Definition newline := String "010" ""%string.
+
+Definition show_map { A :Type} `{_ : Show A} (m : (PMap.t A)) : string :=
+  List.fold_left
+    (fun acc '(key,elt) =>
+       acc ++ (show key) ++ ":" ++ newline
+           ++ (show elt) ++ newline)
+    (PMap.elements m)
+    Coq.Strings.String.EmptyString.
+
+Instance show_map_i  { A :Type} `{_ : Show A} : Show (PMap.t A) :=
+  {| show := show_map |}.
+
+Instance show_component_interface : Show Component.interface :=
   {|
-    show := fun _ => Coq.Strings.String.EmptyString (* TODO *)
+    show := fun ci =>
+              ("Export: ") 
+                ++ (show (Component.export ci)) ++ newline
+                ++ "Import:"
+                ++ (show (Component.import ci)) ++ newline
   |}.
 
-(* TODO implement this *)
-Definition genIntermediateProgram : G Intermediate.program :=
-  let COMP1_ID : positive := 1%positive in
-  let PROC1_ID : positive := 1%positive in
-  let BLOCK1_ID : positive := 1%positive in
-  let component1_interface : Component.interface :=
-      (Component.mkCompInterface [PROC1_ID] []) in
-  let program_interface : Program.interface :=
-      PMap.add COMP1_ID component1_interface (PMap.empty Component.interface) in
-  let buffers := PMap.add COMP1_ID [(BLOCK1_ID,10%nat)] (PMap.empty (list (Block.id * nat))) in
-  let proc1_code := (PMap.add PROC1_ID
-                              ([
-                                  Intermediate.Machine.IConst
-                                    (IPtr (1%positive,1%positive,0%Z) ) R_AUX1 
-                                  ; Intermediate.Machine.IConst (IInt 5%Z) R_AUX2 
-                                  ; Intermediate.Machine.IStore R_AUX1 R_AUX2
-                                  ; Intermediate.Machine.IReturn])
-                              (PMap.empty Intermediate.Machine.code) ) in
-  let procs := PMap.add COMP1_ID proc1_code
-                        (PMap.empty (PMap.t Intermediate.Machine.code)) in
+Instance show_program_interface : Show Program.interface :=
+  {| show := fun pi => show_map pi |}.
+
+Instance show_ptr : Show Pointer.t :=
+  {| show :=
+       fun p => "( cid=" ++ (show (Pointer.component p))
+                      ++ ",bid=" ++ (show (Pointer.block p))
+                      ++ ",off=" ++ (show (Pointer.offset p))
+                      ++ ")"
+  |}.
+
+Instance show_immv : Show imvalue :=
+  {|
+    show :=
+      fun iv =>
+        match iv with
+        | IInt n => "IInt " ++ (show n)
+        | IPtr p => "IPtr " ++ (show p)
+        end
+  |}.
+
+Instance show_register : Show register :=
+  {|
+    show :=
+      fun r =>
+        match r with
+        | R_ONE => "R_ONE"
+        | R_COM => "R_COM"
+        | R_AUX1 => "R_AUX1"
+        | R_AUX2 => "R_AUX2"
+        | R_RA => "R_RA"
+        | R_SP => "R_SP"
+        end
+  |}.
+
+Instance show_binop : Show Common.Values.binop :=
+  {|
+    show :=
+      fun op =>
+        match op with
+        | Common.Values.Add => "+"
+        | Common.Values.Minus => "-"
+        | Common.Values.Mul => "*"
+        | Common.Values.Eq => "="
+        | Common.Values.Leq => "<="
+        end
+  |}.
+
+Instance show_instr : Show Intermediate.Machine.instr :=
+  {| show :=
+       fun i =>
+         match i with
+           | INop => "INop"
+           | ILabel lbl => "ILabel " ++ (show lbl)
+           | IConst v r => "IConst " ++ (show v) ++ " " ++ (show r)
+           | IMov r1 r2 => "IMov " ++ (show r1) ++ " " ++ (show r2)
+           | IBinOp op r1 r2 r3 => "IBinop " ++ (show op)
+                                            ++ " " ++ (show r1)
+                                            ++ " " ++ (show r2)
+                                            ++ " " ++ (show r3)
+           | ILoad r1 r2 => "ILoad " ++ (show r1) ++ " " ++ (show r2)
+           | IStore r1 r2 => "IStore " ++ (show r1) ++ " " ++ (show r2)
+           | IAlloc r1 r2 => "IAlloc " ++ (show r1) ++ " " ++ (show r2)
+           | IBnz r l => "IBnz " ++ (show r) ++ " " ++ (show l)
+           | IJump r => "IJump " ++ (show r)
+           | IJal l => "IJal " ++ (show l) 
+           | ICall cid pid => "ICall " ++ (show cid) ++ " " ++ (show pid)
+           | IReturn => "IReturn"
+           | IHalt => "IHalt"
+         end
+  |}.
+
+Instance show_intermediate_program : Show Intermediate.program :=
+  {|
+    show := fun ip =>
+              ("Interface: ") ++ newline
+                ++ (show (Intermediate.prog_interface ip))
+                ++ ("Buffers: ") ++ newline
+                ++ (show (Intermediate.prog_buffers ip))
+                ++ ("Code: ") ++ newline
+                ++ (show (Intermediate.prog_procedures ip))
+                ++ ("Main: ") ++ newline
+                ++ (show (Intermediate.prog_main ip))
+                         
+  |}.
+
+Theorem label_eq_dec:
+      forall l1 l2 : Intermediate.Machine.label,  {l1 = l2} + {l1 <> l2}.
+    Proof.
+      repeat decide equality. Defined.
+
+(***************************************************************************
+ * Intermediate program generation
+ ***************************************************************************)
+
+Definition choose_pos ( p : positive * positive) :=
+  let Z_to_pos z := (* TODO figure out the proper function to call here *)
+      match z with
+      | Z0 => 1%positive
+      | Zpos p => p
+      | Zneg p => p
+      end in
+  let (lo,hi) := p in 
+  do! p' <- choose (Zpos lo, Zpos hi);
+    returnGen (Z_to_pos p').
+
+Definition pos_list (l : nat) : list positive :=
+  List.map Pos.of_nat (List.seq 1 l).
+
+Definition gen_pair_list {A B : Type} (ga : G (list A)) (gb : G (list B)) : G (list (A*B)) :=
+  liftGen (fun '(la,lb) => List.combine la lb) 
+          (liftGen2 pair ga gb).
+
+Definition gen_sublist {A : Type} ( default : A ) ( all : list A ) : G (list A) :=
+  match all with
+  | [] => returnGen []
+  | _ => 
+    do! n <- (choose (1%nat,(List.length all)));
+      (vectorOf n (elements default all))
+  end.
+    
+Definition gen_program_interface (cids : list Component.id) : G Program.interface :=
+  let proc_ids := do! n <- choose(1%nat,5%nat); returnGen (pos_list n) in
+  do! exported_procs <- (vectorOf (List.length cids) proc_ids);
+  let all_procs := List.flat_map
+                     (fun '(cid,lp) => List.map (fun pid => (cid,pid)) lp)
+                     (List.combine cids exported_procs) in
+  do! imported_procs <-  
+    sequenceGen (
+      List.map (fun cid =>
+                  do! import_procs <- (gen_sublist (1%positive,1%positive) all_procs);
+                    returnGen (List.filter (fun '(cid',_) =>
+                                              negb (Pos.eqb cid cid'))
+                                           (List.nodup procs_eqdec import_procs))  
+               ) cids);
+  returnGen (PMapExtra.of_list
+               (List.combine
+                  cids 
+                  (List.map
+                     (fun '(e,i) => (Component.mkCompInterface e i))
+                     (List.combine exported_procs imported_procs)
+                  )
+               )
+            ).
+
+Definition gen_buffers (cids : list Component.id) : G (PMap.t (list (Block.id * nat))) :=
+  let gen_n_buffers : G (list (Block.id * nat)) :=
+      do! n <- arbitrary; 
+        let ids := pos_list n in
+        do! sizes <- vectorOf n (choose (1%nat, N.to_nat (SFI.SLOT_SIZE-1)%N));
+          returnGen (List.combine ids sizes) in
+  do! buffers <- (vectorOf (List.length cids) gen_n_buffers);
+    returnGen (PMapExtra.of_list (List.combine cids buffers)).
+
+Section CodeGeneration.
+
+  Variable pi : Program.interface.
+
+  Variable buffers : PMap.t (list (Block.id * nat)).
+
+  Variable cid : Component.id.
+
+  Variable pid : Procedure.id.
+  
+  Instance genOp : Gen Common.Values.binop :=
+    {
+      arbitrary := elems [
+                       Common.Values.Add 
+                       ; Common.Values.Minus 
+                       ; Common.Values.Mul 
+                       ; Common.Values.Eq 
+                       ; Common.Values.Leq 
+                     ]
+    }.
+
+  Instance genRegs : Gen Intermediate.Machine.register :=
+    {
+      arbitrary := elems [
+                       R_ONE
+                       ; R_COM
+                       ; R_AUX1
+                       ; R_AUX2
+                       ; R_RA
+                       ; R_SP
+                     ]
+    }.
+
+ 
+  Definition genPtrImVal : G (option Intermediate.Machine.imvalue) :=
+    let  genPointer (id : Component.id) :=
+         match PMap.find id buffers with
+         | None => returnGen None
+         | Some blocks =>
+           do! b <- elements (None) (List.map Some blocks);
+             match b with
+             | None => returnGen None
+             | Some (bid,size) =>
+               do! offset <- choose (Z0,Z.of_nat size);
+                 returnGen (Some (Intermediate.Machine.IPtr ((cid,bid),offset) ))
+             end
+         end in    
+    backtrack [
+        ( 4%nat, (genPointer cid) )
+        ; ( 1%nat,
+            (do! id <- (elements (1%positive) (List.map fst (PMap.elements pi)));
+               (genPointer id)))
+      ].
+
+   
+  Definition genIntImVal : G Intermediate.Machine.imvalue :=
+    do! n<-arbitrary; returnGen (Intermediate.Machine.IInt n).
+  
+
+  Definition genImVal : G imvalue :=
+    let genImValAux : G Intermediate.Machine.imvalue :=    
+        do! res <- genPtrImVal;
+          match res with
+          | None => genIntImVal
+          | Some ptr => returnGen ptr
+          end in 
+    freq
+      [ (4%nat, genIntImVal)
+        ; (1%nat, genImValAux) ].
+
+  Definition genIConst : G instr :=
+    do! v <- genIntImVal;
+      do! r <- arbitrary;
+      returnGen (IConst v r).
+
+  Definition gen2Reg (it :  register -> register -> instr) : G instr :=
+    do! r1 <- arbitrary;
+      do! r2 <- arbitrary;
+      returnGen (it r1 r2).
+
+  Definition genIBinOp : G instr :=
+    do! op <- arbitrary;
+      do! r1 <- arbitrary;
+      do! r2 <- arbitrary;
+      do! r3 <- arbitrary;
+      returnGen (IBinOp op r1 r2 r3).
+
+
+  Definition genIJump : G instr :=
+    do! r <- arbitrary;
+      returnGen (IJump r).
+
+  Definition genICall : G instr :=
+    match PMap.find cid pi with
+    | None => returnGen INop (* This should not happen *)
+    | Some comp_interface =>
+      let imports := (Component.import comp_interface) in
+      match imports with
+      | nil => returnGen INop (* no imports; can't generate ICall *)
+      | (cid1,pid1)::xs =>
+        do! p <- elements (cid1,pid1) imports;
+          let (cid',pid') := p in
+          returnGen (ICall cid' pid')
+      end
+    end.
+                                                            
+  Definition genIBnz (first_label : positive) (lbl : positive) : G instr :=
+    do! r <- arbitrary;
+      if (Pos.ltb first_label (lbl+3))%positive
+      then
+        do! target <- choose_pos (first_label,(lbl+3)%positive);
+          returnGen (IBnz r target)
+      else
+        do! target <- choose_pos (lbl,(lbl+3)%positive);
+          returnGen (IBnz r target).
+      
+  Definition genILabel (lbl : positive) : G instr :=
+    returnGen (ILabel lbl).
+
+  Definition gen_procedure (next_label : positive) : G code :=
+    let get_missing_labels proc :=
+        let decl := List.map (fun i =>
+                                match i with
+                                | ILabel l => l
+                                | _ => 1%positive (* this is not happening *)
+                                end
+                             )
+                             (List.filter (fun i => match i with
+                                                 | ILabel _ => true
+                                                 | _ => false
+                                                 end ) proc ) in
+        let uses :=  List.map (fun i =>
+                                match i with
+                                | IBnz _ l => l
+                                | _ => 1%positive (* this is not happening *)
+                                end
+                             )
+                             (List.filter (fun i => match i with
+                                                 | IBnz _ _ => true
+                                                 | _ => false
+                                                 end ) proc ) in
+        List.nodup label_eq_dec
+                   (List.filter (fun l => Nat.eqb 0%nat (List.count_occ label_eq_dec decl l))
+                                uses)
+    in
+        
+  let gen_instr  (first_label : positive)  (next_label : positive) :=
+      freq [
+          (1%nat,(returnGen INop))
+          ; (4%nat, genIConst)
+          ; (4%nat, genILabel next_label) 
+          ; (4%nat, gen2Reg IMov)
+          ; (7%nat, genIBinOp)
+          ; (4%nat, gen2Reg ILoad)
+          ; (4%nat, gen2Reg IStore)
+          ; (4%nat, genIBnz first_label next_label)
+          ; (4%nat, genIJump)
+          (* ; (4%nat, genIJal) *)
+          ; (4%nat, genICall)
+          ; (4%nat, gen2Reg IAlloc)
+          ; (1%nat, (returnGen IHalt))
+          ; (1%nat, (returnGen IReturn))
+        ] in
+  let fix aux proc len first_lbl lbl :=
+      match len with
+      | O => 
+        returnGen (proc
+                     (* generate missing labels *) 
+                     ++ (List.map (fun l => ILabel l) (get_missing_labels proc))
+                     ++ [IReturn])%list
+      | S len' =>
+        do! i <- gen_instr first_lbl lbl;
+          match i with
+          | ILabel _ => aux (proc ++ [i])%list len' first_lbl (lbl+1)%positive
+          | IReturn | IHalt =>
+                      returnGen (proc
+                                   (* generate missing labels *) 
+                                   ++ (List.map (fun l => ILabel l) (get_missing_labels proc))
+                                   ++ [i])%list
+          | _ => aux (proc ++ [i])%list len' first_lbl lbl
+          end
+      end in
+  aux [] 10%nat next_label next_label.
+    
+
+End CodeGeneration.
+
+Definition gen_procs (pi : Program.interface) (buffers : PMap.t (list (Block.id * nat))) : G (PMap.t (PMap.t code)) :=
+  let max_label (procs : PMap.t code) :=
+      PMap.fold (fun _ proc acc =>
+                   (List.fold_left (fun acc' i =>
+                                match i with
+                                | ILabel l => if (Pos.ltb acc' l) then l else acc'
+                                | _ => acc'
+                                end
+                             ) proc acc)
+                ) procs 1%positive
+  in
+  foldGen
+    (fun acc '(cid,comp_interface) =>
+       do! proc_map <- (
+           foldGen
+             (fun acc pid =>
+                do! proc <- gen_procedure pi cid ((max_label acc) + 1)%positive;
+                returnGen (PMap.add pid proc acc)
+             ) (Component.export comp_interface) (PMap.empty code));       
+       returnGen (PMap.add cid proc_map acc)
+    ) (PMap.elements pi)
+    (PMap.empty (PMap.t code))
+.
+
+Definition gen_main (pi : Program.interface) : G (Component.id * Procedure.id) :=
+  do! cid <- elements 1%positive (List.map fst (PMap.elements pi));
+    match PMap.find cid pi with
+    | None => returnGen (cid,1%positive)
+    | Some cint => do! pid <- elements 1%positive (Component.export cint);
+                   returnGen (cid,pid)
+    end.
+  
+
+  (* TODO implement this *)
+  Definition genIntermediateProgram : G Intermediate.program :=
+    do! n <- choose (1%nat, (N.to_nat (SFI.COMP_MAX-1)%N));
+      let cids : list Component.id := pos_list n in
+  
+  do! program_interface <- (gen_program_interface cids);
+  do! buffers <- (gen_buffers cids);
+  do! procs <- gen_procs program_interface buffers;
+  do! main <- gen_main program_interface;
   returnGen {|
         Intermediate.prog_interface := program_interface;
         Intermediate.prog_procedures := procs;
         Intermediate.prog_buffers := buffers;
-        Intermediate.prog_main := (COMP1_ID,PROC1_ID)
+        Intermediate.prog_main := main
       |}.
 
 
@@ -91,7 +479,7 @@ Conjecture correct_data_compartmentalized:
 
     
 (************************************************
- * No writes outside it's own memory, 
+ * No writes outside its own memory, 
  * except for push sfi.
  *************************************************)
 
@@ -157,7 +545,8 @@ Definition store_correct : Checker :=
   forAll genIntermediateProgram
   ( fun ip =>
       match compile_program ip with
-      | TargetSFI.EitherMonad.Left msg => checker false
+      | TargetSFI.EitherMonad.Left msg =>
+        whenFail ("Compilation error: " ++ msg) false
       | TargetSFI.EitherMonad.Right p =>
         let (res,log) := eval_store_program p in
         store_checker log (* check the log even if the program fails *)
@@ -237,7 +626,8 @@ Definition jump_correct : Checker :=
   forAll genIntermediateProgram
          ( fun ip =>
              match compile_program ip with
-             | TargetSFI.EitherMonad.Left msg => checker false
+             | TargetSFI.EitherMonad.Left msg =>
+               whenFail ("Compilation error: " ++ msg) false
              | TargetSFI.EitherMonad.Right p =>
                let (res,log) := eval_jump_program p in
                jump_checker log (* check the log even if the program fails *)
@@ -351,7 +741,8 @@ Definition cs_correct : Checker :=
   forAll genIntermediateProgram
          ( fun ip =>
              match compile_program ip with
-             | TargetSFI.EitherMonad.Left msg => checker false
+             | TargetSFI.EitherMonad.Left msg =>
+               whenFail ("Compilation error: " ++ msg) false
              | TargetSFI.EitherMonad.Right p =>
                let (res,log) := eval_cs_program p in
                match res with
@@ -368,11 +759,4 @@ QuickChick store_correct.
 QuickChick jump_correct.
 QuickChick cs_correct.
 
-(* test compile correctness *)
-
-(* Conjecture robust_compilation : *)
-(*   forall (ip : Intermediate.program) (sp : sfi_program) *)
-(*     (sc : sfi_program) (b : trace) *)
-
-(*     eval  *)
-(* . *)
+(* TODO test compile correctness *)
